Develop wheatLang and its semantics

pancake/semantics/wheatSemScript.sml
@@ -18,20 +18,18 @@ Datatype:
   state =
     <| locals  : ('a word_loc) num_map
      ; globals : 5 word  |-> 'a word_loc
-     ; fp_regs : num |-> word64 (* FP regs are treated "globally" *)
      ; memory  : 'a word -> 'a word_loc
      ; mdomain : ('a word) set
      ; clock   : num
-     ; code    : (num # ('a wheatLang$prog)) num_map
+     ; code    : (num list # ('a wheatLang$prog)) num_map
      ; be      : bool
      ; ffi     : 'ffi ffi_state |>
 End
 
-
 val state_component_equality = theorem "state_component_equality";
 
 Datatype:
-  result = Result    ('w word_loc) (* TODISC: keeping the wordSem's name (Result) for Return *)
+  result = Result    ('w word_loc)
          | Exception ('w word_loc)
          | Break
          | Continue
@@ -39,7 +37,6 @@ Datatype:
          | FinalFFI final_event
          | Error
 End
-
 
 val s = ``(s:('a,'ffi) wheatSem$state)``
 
@@ -53,7 +50,6 @@ Definition fix_clock_def:
       <| clock := if old_s.clock < new_s.clock then old_s.clock else new_s.clock |>)
 End
 
-(* gv: global variable *)
 Definition set_globals_def:
   set_globals gv w ^s =
     (s with globals := s.globals |+ (gv,w))
@@ -95,7 +91,6 @@ Termination
    \\ DECIDE_TAC)
 End
 
-
 Definition get_vars_def:
   (get_vars [] ^s = SOME []) /\
   (get_vars (v::vs) s =
@@ -116,26 +111,25 @@ Definition set_vars_def:
   (s with locals := (alist_insert vs xs s.locals))
 End
 
-(* TODISC: not using find_code from wordSem as it additionally takes stack_size *)
 Definition find_code_def:
   (find_code (SOME p) args code =
      case sptree$lookup p code of
      | NONE => NONE
-     | SOME (arity,exp) => if LENGTH args = arity then SOME (args,exp)
-                                                    else NONE) /\
+     | SOME (params,exp) => if LENGTH args = LENGTH params
+                            then SOME (fromAList (ZIP (params, args)),exp) else NONE) /\
   (find_code NONE args code =
      if args = [] then NONE else
        case LAST args of
        | Loc loc 0 =>
            (case lookup loc code of
             | NONE => NONE
-            | SOME (arity,exp) => if LENGTH args = arity + 1
-                                  then SOME (FRONT args,exp)
-                                  else NONE)
+            | SOME (params,exp) => if LENGTH args = LENGTH params + 1
+                                   then SOME (fromAList (ZIP (params, FRONT args)),exp)
+                                   else NONE)
       | other => NONE)
 End
 
-
+(*
 Definition to_wheat_state_def:
   to_wheat_state (s:('a, 'b, 'c) wordSem$state)  =
     <| locals  := s.locals
@@ -148,7 +142,6 @@ Definition to_wheat_state_def:
      ; be      := s.be
      ; ffi     := s.ffi |>
 End
-
 
 Definition to_word_state_def:
   to_word_state s =
@@ -185,7 +178,7 @@ Definition inst_wrapper_def:
     | SOME s' => SOME ((f s') : ('a, 'b) wheatSem$state)
     | NONE => NONE
 End
-
+*)
 
 Definition get_var_imm_def:
   (get_var_imm ((Reg n):'a reg_imm) ^s = sptree$lookup n s.locals) ∧
@@ -202,6 +195,13 @@ QED
 Definition call_env_def:
   call_env args ^s =
     s with <| locals := fromList args |>
+End
+
+Definition cut_state_def:
+  cut_state live s =
+    if domain live SUBSET domain s.locals then
+      SOME (s with locals := inter s.locals live)
+    else NONE
 End
 
 Definition evaluate_def:
@@ -228,10 +228,7 @@ Definition evaluate_def:
     case eval s src of
      | SOME w => (NONE, set_globals dst w s)
      | _ => (SOME Error, s)) /\
-  (evaluate (Inst i,s) =
-     case ARB (*inst_wrapper i to_wheat_state s *)  of
-     | SOME s1 => (NONE, s1)
-     | NONE => (SOME Error, s)) /\
+  (evaluate (LoadByte dst src,s) = (SOME Error, s)) /\
   (evaluate (Seq c1 c2,s) =
      let (res,s1) = fix_clock s (evaluate (c1,s)) in
      if res = NONE then evaluate (c2,s1) else (res,s1)) /\
@@ -241,9 +238,23 @@ Definition evaluate_def:
       if word_cmp cmp x y then evaluate (c1,s)
                           else evaluate (c2,s)
     | _ => (SOME Error,s))) /\
+  (evaluate (Mark p,s) = evaluate (p,s)) /\
   (evaluate (Break,s) = (SOME Break,s)) /\
   (evaluate (Continue,s) = (SOME Continue,s)) /\
-  (evaluate (While cmp r1 ri c,s) = ARB) /\
+  (evaluate (Loop live_in body live_out,s) =
+    (case cut_state live_in s of
+     | SOME s =>
+        (let (res,s1) = fix_clock s (evaluate (body,s)) in
+           if s1.clock = 0 then (SOME TimeOut,s1) else
+             case res of
+             | NONE => evaluate (Loop live_in body live_out,dec_clock s1)
+             | SOME Continue => evaluate (Loop live_in body live_out,dec_clock s1)
+             | SOME Break =>
+                 (case cut_state live_out s1 of
+                  | SOME s2 => (NONE,s2)
+                  | NONE => (SOME Error,s1))
+             | _ => (res,s1))
+     | _ => (SOME Error,s))) /\
   (evaluate (Raise n,s) =
      case lookup n s.locals of
      | NONE => (SOME Error,s)
@@ -263,30 +274,32 @@ Definition evaluate_def:
     case get_vars argvars s of
     | NONE => (SOME Error,s)
     | SOME argvals =>
-      if (dest = NONE /\ argvals = []) then (SOME Error,s)
-      else
-        case find_code dest argvals s.code of
+       (case find_code dest argvals s.code of
         | NONE => (SOME Error,s)
-        | SOME (args,prog) =>
-          case ret of
+        | SOME (env,prog) =>
+         (case ret of
           | NONE (* tail call *) =>
-            if handler = NONE then
-             if s.clock = 0 then (SOME TimeOut,call_env [] s)
-             else (case evaluate (prog, call_env args (dec_clock s)) of
-                    | (NONE,s) => (SOME Error,s)
-                    | (SOME res,s) => (SOME res,s))
-           else (SOME Error,s) (* tail-call requires no handler *)
-          | SOME n (* returning call, returns into var n *) =>
-              if s.clock = 0 then (SOME TimeOut,call_env [] s)
-              else (case fix_clock (call_env args (dec_clock s))
-                                   (evaluate (prog, call_env args (dec_clock s))) of
-                      | (NONE,st) => (SOME Error,st)
-                      | (SOME (Result retv),st) => (NONE, set_var n retv st)
-                      | (SOME (Exception exn),st) =>
-                          (case handler of (* if handler is present, then handle exc *)
-                            | NONE => (SOME (Exception exn),st)
-                            | SOME (n,h) => evaluate (h, set_var n exn st))
-                          | res => res)) /\
+            (if handler <> NONE then (SOME Error,s) else
+               if s.clock = 0 then (SOME TimeOut,s)
+               else (case evaluate (prog, dec_clock s with locals := env) of
+                     | (NONE,s) => (SOME Error,s)
+                     | (SOME res,s) => (SOME res,s)))
+          | SOME (n,live) =>
+            (case cut_state live s of
+             | NONE => (SOME Error,s)
+             | SOME s =>
+               if s.clock = 0 then (SOME TimeOut,s) else
+                 (case fix_clock (dec_clock s with locals := env)
+                            (evaluate (prog, dec_clock s with locals := env))
+                   of (NONE,st) => (SOME Error,(st with locals := s.locals))
+                    | (SOME (Result retv),st) =>
+                        (NONE, set_var n retv (st with locals := s.locals))
+                    | (SOME (Exception exn),st) =>
+                        (case handler of (* if handler is present, then handle exc *)
+                         | NONE => (SOME (Exception exn),(st with locals := s.locals))
+                         | SOME (n,h) =>
+                             evaluate (h, set_var n exn (st with locals := s.locals)))
+                    | res => res))))) /\
   (evaluate (FFI ffi_index ptr1 len1 ptr2 len2,s) =
     case (lookup len1 s.locals, lookup ptr1 s.locals, lookup len2 s.locals, lookup ptr2 s.locals) of
     | SOME (Word w),SOME (Word w2),SOME (Word w3),SOME (Word w4) =>
@@ -310,349 +323,40 @@ Termination
   \\ imp_res_tac (GSYM fix_clock_IMP_LESS_EQ)
   \\ full_simp_tac(srw_ss())[set_var_def,call_env_def,dec_clock_def,set_globals_def,LET_THM]
   \\ rpt (pairarg_tac \\ full_simp_tac(srw_ss())[])
-  \\ every_case_tac \\ full_simp_tac(srw_ss())[]
+  \\ fs [cut_state_def]
+  \\ every_case_tac \\ rveq \\ full_simp_tac(srw_ss())[]
   \\ decide_tac
 End
 
-
-val evaluate_ind = theorem"evaluate_ind";
-
-
-(*
-remove_it_later: leaving it here to check TOCHECK notes *)
-(*Definition inst_def:
-  inst i ^s =
-    case i of
-    | Skip => SOME s
-    | Const reg w => assign reg (Const w) s
-    | Arith (Binop bop r1 r2 ri) =>
-        assign r1
-          (Op bop [Var r2; case ri of Reg r3 => Var r3
-                                    | Imm w => Const w]) s
-    | Arith (Shift sh r1 r2 n) =>
-        assign r1
-        (Shift sh (Var r2) n) s
-    | Arith (Div r1 r2 r3) =>
-       (let vs = get_vars[r3;r2] s in
-       case vs of
-       SOME [Word q;Word w2] =>
-         if q ≠ 0w then
-           SOME (set_var r1 (Word (w2 / q)) s)
-         else NONE
-       | _ => NONE)
-    | Arith (AddCarry r1 r2 r3 r4) =>
-        (let vs = get_vars [r2;r3;r4] s in
-        case vs of
-        SOME [Word l;Word r;Word c] =>
-          let res = w2n l + w2n r + if c = (0w:'a word) then 0 else 1 in
-            SOME (set_var r4 (Word (if dimword(:'a) ≤ res then (1w:'a word) else 0w))
-                 (set_var r1 (Word (n2w res)) s))
-
-        | _ => NONE)
-    | Arith (AddOverflow r1 r2 r3 r4) =>
-        (let vs = get_vars [r2;r3] s in
-        case vs of
-        SOME [Word w2;Word w3] =>
-          SOME (set_var r4 (Word (if w2i (w2 + w3) ≠ w2i w2 + w2i w3 then 1w else 0w))
-                 (set_var r1 (Word (w2 + w3)) s))
-        | _ => NONE)
-    | Arith (SubOverflow r1 r2 r3 r4) =>
-        (let vs = get_vars [r2;r3] s in
-        case vs of
-        SOME [Word w2;Word w3] =>
-          SOME (set_var r4 (Word (if w2i (w2 - w3) ≠ w2i w2 - w2i w3 then 1w else 0w))
-                 (set_var r1 (Word (w2 - w3)) s))
-        | _ => NONE)
-    | Arith (LongMul r1 r2 r3 r4) =>
-        (let vs = get_vars [r3;r4] s in
-        case vs of
-        SOME [Word w3;Word w4] =>
-         let r = w2n w3 * w2n w4 in
-           SOME (set_var r2 (Word (n2w r)) (set_var r1 (Word (n2w (r DIV dimword(:'a)))) s))
-        | _ => NONE)
-   | Arith (LongDiv r1 r2 r3 r4 r5) =>
-       (let vs = get_vars [r3;r4;r5] s in
-       case vs of
-       SOME [Word w3;Word w4;Word w5] =>
-         let n = w2n w3 * dimword (:'a) + w2n w4 in
-         let d = w2n w5 in
-         let q = n DIV d in
-         if (d ≠ 0 ∧ q < dimword(:'a)) then
-           SOME (set_var r1 (Word (n2w q)) (set_var r2 (Word (n2w (n MOD d))) s))
-         else NONE
-      | _ => NONE)
-    | Mem Load r (Addr a w) =>
-       (case eval s (Op Add [Var a; Const w]) of
-        | SOME (Word w) =>
-           (case mem_load w s of
-            | NONE => NONE
-            | SOME w => SOME (set_var r w s))
-        | _ => NONE)
-    | Mem Load8 r (Addr a w) =>
-       (case eval s (Op Add [Var a; Const w]) of
-        | SOME (Word w) =>
-           (case mem_load_byte_aux s.memory s.mdomain s.be w of
-            | NONE => NONE
-            | SOME w => SOME (set_var r (Word (w2w w)) s))
-           | _ => NONE)
-    | Mem Store r (Addr a w) =>
-       (case (eval s (Op Add [Var a; Const w]), lookup r s.locals) of
-        | (SOME (Word a), SOME w) =>
-            (case mem_store a w s of
-             | SOME s1 => SOME s1
-             | NONE => NONE)
-        | _ => NONE)
-    | Mem Store8 r (Addr a w) =>
-       (case (eval s (Op Add [Var a; Const w]), lookup r s.locals) of
-        | (SOME (Word a), SOME (Word w)) =>
-            (case mem_store_byte_aux s.memory s.mdomain s.be a (w2w w) of
-             | SOME new_m => SOME (s with memory := new_m)
-             | NONE => NONE)
-        | _ => NONE)
-    | FP (FPLess r d1 d2) =>
-      (case (get_fp_var d1 s,get_fp_var d2 s) of
-      | (SOME f1 ,SOME f2) =>
-        SOME (set_var r
-          (Word (if fp64_lessThan f1 f2
-                 then 1w
-                 else 0w)) s)
-      | _ => NONE)
-    | FP (FPLessEqual r d1 d2) =>
-      (case (get_fp_var d1 s,get_fp_var d2 s) of
-      | (SOME f1, SOME f2) =>
-        SOME (set_var r
-          (Word (if fp64_lessEqual f1 f2
-                 then 1w
-                 else 0w)) s)
-      | _ => NONE)
-    | FP (FPEqual r d1 d2) =>
-      (case (get_fp_var d1 s,get_fp_var d2 s) of
-      | (SOME f1, SOME f2) =>
-        SOME (set_var r
-          (Word (if fp64_equal f1 f2
-                 then 1w
-                 else 0w)) s)
-      | _ => NONE)
-    | FP (FPMov d1 d2) =>
-      (case get_fp_var d2 s of
-      | SOME f =>
-        SOME (set_fp_var d1 f s)
-      | _ => NONE)
-    | FP (FPAbs d1 d2) =>
-      (case get_fp_var d2 s of
-      | SOME f =>
-        SOME (set_fp_var d1 (fp64_abs f) s)
-      | _ => NONE)
-    | FP (FPNeg d1 d2) =>
-      (case get_fp_var d2 s of
-      | SOME f =>
-        SOME (set_fp_var d1 (fp64_negate f) s)
-      | _ => NONE)
-    | FP (FPSqrt d1 d2) =>
-      (case get_fp_var d2 s of
-      | SOME f =>
-        SOME (set_fp_var d1 (fp64_sqrt roundTiesToEven f) s)
-      | _ => NONE)
-    | FP (FPAdd d1 d2 d3) =>
-      (case (get_fp_var d2 s,get_fp_var d3 s) of
-      | (SOME f1,SOME f2) =>
-        SOME (set_fp_var d1 (fp64_add roundTiesToEven f1 f2) s)
-      | _ => NONE)
-    | FP (FPSub d1 d2 d3) =>
-      (case (get_fp_var d2 s,get_fp_var d3 s) of
-      | (SOME f1,SOME f2) =>
-        SOME (set_fp_var d1 (fp64_sub roundTiesToEven f1 f2) s)
-      | _ => NONE)
-    | FP (FPMul d1 d2 d3) =>
-      (case (get_fp_var d2 s,get_fp_var d3 s) of
-      | (SOME f1,SOME f2) =>
-        SOME (set_fp_var d1 (fp64_mul roundTiesToEven f1 f2) s)
-      | _ => NONE)
-    | FP (FPDiv d1 d2 d3) =>
-      (case (get_fp_var d2 s,get_fp_var d3 s) of
-      | (SOME f1,SOME f2) =>
-        SOME (set_fp_var d1 (fp64_div roundTiesToEven f1 f2) s)
-      | _ => NONE)
-    | FP (FPFma d1 d2 d3) =>
-      (case (get_fp_var d1 s, get_fp_var d2 s, get_fp_var d3 s) of
-      | (SOME f1, SOME f2, SOME f3) =>
-        SOME (set_fp_var d1 (fpSem$fpfma f1 f2 f3) s)
-      | _ => NONE)
-    | FP (FPMovToReg r1 r2 d) =>
-      (case get_fp_var d s of
-      | SOME v =>
-        if dimindex(:'a) = 64 then
-          SOME (set_var r1 (Word (w2w v)) s)
-        else
-          SOME (set_var r2 (Word ((63 >< 32) v)) (set_var r1 (Word ((31 >< 0) v)) s))
-      | _ => NONE)
-    | FP (FPMovFromReg d r1 r2) =>
-      (if dimindex(:'a) = 64 then
-        case lookup r1 s.locals of
-          SOME (Word w1) => SOME (set_fp_var d (w2w w1) s)
-        | _ => NONE
-      else
-        case (lookup r1 s.locals,lookup r2 s.locals) of
-          (SOME (Word w1),SOME (Word w2)) => SOME (set_fp_var d (w2 @@ w1) s)
-        | _ => NONE)
-    | FP (FPToInt d1 d2) =>
-      (case get_fp_var d2 s of
-        NONE => NONE
-      | SOME f =>
-      case fp64_to_int roundTiesToEven f of
-        NONE => NONE
-      | SOME i =>
-        let w = i2w i : word32 in
-        if w2i w = i then
-          (if dimindex(:'a) = 64 then
-             SOME (set_fp_var d1 (w2w w) s)
-           else
-           case get_fp_var (d1 DIV 2) s of
-             NONE => NONE
-           | SOME f =>
-             let (h, l) = if ODD d1 then (63, 32) else (31, 0) in
-                  SOME (set_fp_var (d1 DIV 2) (bit_field_insert h l w f) s))
-        else
-          NONE)
-    | FP (FPFromInt d1 d2) =>
-      if dimindex(:'a) = 64 then
-        case get_fp_var d2 s of
-        | SOME f =>
-          let i =  w2i ((31 >< 0) f : word32) in
-            SOME (set_fp_var d1 (int_to_fp64 roundTiesToEven i) s)
-        | NONE => NONE
-      else
-        case get_fp_var (d2 DIV 2) s of
-        | SOME v =>
-          let i =  w2i (if ODD d2 then (63 >< 32) v else (31 >< 0) v : 'a word) in
-            SOME (set_fp_var d1 (int_to_fp64 roundTiesToEven i) s)
-        | NONE => NONE
-    | _ => NONE
-End
-
-*)
-
-
-(*
-(* We prove that the clock never increases and that termdep is constant. *)
-
-Theorem gc_clock:
-   !s1 s2. (gc s1 = SOME s2) ==> s2.clock <= s1.clock /\ s2.termdep = s1.termdep
-Proof
-  full_simp_tac(srw_ss())[gc_def,LET_DEF] \\ SRW_TAC [] []
-  \\ every_case_tac >> full_simp_tac(srw_ss())[]
-  \\ SRW_TAC [] [] \\ full_simp_tac(srw_ss())[]
-QED
-
-Theorem alloc_clock:
-   !xs s1 vs s2. (alloc x names s1 = (vs,s2)) ==>
-                  s2.clock <= s1.clock /\ s2.termdep = s1.termdep
-Proof
-  SIMP_TAC std_ss [alloc_def] \\ rpt gen_tac
-  \\ rpt (BasicProvers.TOP_CASE_TAC \\ full_simp_tac(srw_ss())[])
-  \\ imp_res_tac gc_clock
-  \\ rpt (disch_then strip_assume_tac)
-  \\ rpt var_eq_tac \\ full_simp_tac(srw_ss())[]
-  \\ full_simp_tac(srw_ss())[push_env_def,set_store_def,call_env_def
-                            ,LET_THM,pop_env_def,flush_state_def]
-  \\ rpt (pairarg_tac \\ full_simp_tac(srw_ss())[])
-  \\ every_case_tac \\ full_simp_tac(srw_ss())[]
-  \\ rpt var_eq_tac \\ full_simp_tac(srw_ss())[]
-QED
-
-val inst_clock = Q.prove(
-  `inst i s = SOME s2 ==> s2.clock <= s.clock /\ s2.termdep = s.termdep`,
-  Cases_on `i` \\ full_simp_tac(srw_ss())[inst_def,assign_def,get_vars_def,LET_THM]
-  \\ every_case_tac
-  \\ SRW_TAC [] [set_var_def] \\ full_simp_tac(srw_ss())[]
-  \\ full_simp_tac(srw_ss())[mem_store_def] \\ SRW_TAC [] []
-  \\ EVAL_TAC \\ fs[]);
+(* We prove that the clock never increases *)
 
 Theorem evaluate_clock:
-   !xs s1 vs s2. (evaluate (xs,s1) = (vs,s2)) ==>
-                 s2.clock <= s1.clock /\ s2.termdep = s1.termdep
+  !xs s1 vs s2. (evaluate (xs,s1) = (vs,s2)) ==> s2.clock <= s1.clock
 Proof
-  recInduct evaluate_ind \\ REPEAT STRIP_TAC
-  \\ POP_ASSUM MP_TAC \\ ONCE_REWRITE_TAC [evaluate_def]
+  recInduct evaluate_ind \\ rpt strip_tac
+  \\ pop_assum mp_tac \\ once_rewrite_tac [evaluate_def]
   \\ rpt (disch_then strip_assume_tac)
-  \\ full_simp_tac(srw_ss())[] \\ rpt var_eq_tac \\ full_simp_tac(srw_ss())[]
-  \\ rpt (pop_assum mp_tac)
-  \\ rpt (BasicProvers.TOP_CASE_TAC \\ full_simp_tac(srw_ss())[])
-  \\ rpt (disch_then strip_assume_tac)
-  \\ imp_res_tac alloc_clock \\ full_simp_tac(srw_ss())[]
-  \\ rpt var_eq_tac \\ full_simp_tac(srw_ss())[]
-  \\ full_simp_tac(srw_ss())[set_vars_def,set_var_def,set_store_def]
-  \\ imp_res_tac inst_clock \\ full_simp_tac(srw_ss())[]
-  \\ full_simp_tac(srw_ss())[mem_store_def,call_env_def,dec_clock_def,flush_state_def]
-  \\ rpt var_eq_tac \\ full_simp_tac(srw_ss())[]
-  \\ full_simp_tac(srw_ss())[LET_THM] \\ rpt (pairarg_tac \\ full_simp_tac(srw_ss())[])
-  \\ full_simp_tac(srw_ss())[jump_exc_def,pop_env_def]
-  \\ every_case_tac \\ full_simp_tac(srw_ss())[]
-  \\ rpt var_eq_tac \\ full_simp_tac(srw_ss())[]
-  \\ imp_res_tac fix_clock_IMP_LESS_EQ \\ full_simp_tac(srw_ss())[]
-  \\ imp_res_tac LESS_EQ_TRANS \\ full_simp_tac(srw_ss())[]
-  \\ TRY (Cases_on `handler`)
-  \\ TRY (PairCases_on `x`)
-  \\ TRY (PairCases_on `x''`)
-  \\ full_simp_tac(srw_ss())[push_env_def,LET_THM]
-  \\ rpt (pairarg_tac \\ full_simp_tac(srw_ss())[])
-  \\ decide_tac
+  \\ fs [] \\ rveq \\ fs []
+  \\ fs [CaseEq"option",CaseEq"word_loc",mem_store_def,CaseEq"bool",
+         cut_state_def,pair_case_eq,CaseEq"ffi_result"]
+  \\ fs [] \\ rveq \\ fs [set_var_def,set_globals_def,dec_clock_def,call_env_def]
+  \\ rpt (pairarg_tac \\ fs [])
+  \\ fs [CaseEq"option",CaseEq"word_loc",mem_store_def,CaseEq"bool",CaseEq"result",
+         pair_case_eq]
+  \\ fs [] \\ rveq \\ fs [set_var_def,set_globals_def]
+  \\ imp_res_tac fix_clock_IMP_LESS_EQ \\ fs []
 QED
 
-val fix_clock_evaluate = Q.prove(
-  `fix_clock s (evaluate (c1,s)) = evaluate (c1,s)`,
-  Cases_on `evaluate (c1,s)` \\ full_simp_tac(srw_ss())[fix_clock_def]
-  \\ imp_res_tac evaluate_clock \\ full_simp_tac(srw_ss())[GSYM NOT_LESS]
-  \\ full_simp_tac(srw_ss())[state_component_equality]);
+Theorem fix_clock_evaluate:
+  fix_clock s (evaluate (c1,s)) = evaluate (c1,s)
+Proof
+  Cases_on ‘evaluate (c1,s)’ \\ rw [fix_clock_def]
+  \\ imp_res_tac evaluate_clock \\ fs [state_component_equality]
+QED
 
 (* We store the theorems without fix_clock *)
 
-val evaluate_ind = save_thm("evaluate_ind",
-  REWRITE_RULE [fix_clock_evaluate] evaluate_ind);
-
-val evaluate_def = save_thm("evaluate_def[compute]",
-  REWRITE_RULE [fix_clock_evaluate] evaluate_def);
-
-(* observational semantics *)
-
-val semantics_def = Define `
-  semantics ^s start =
-  let prog = Call NONE (SOME start) [0] NONE in
-  if ∃k. case FST(evaluate (prog,s with clock := k)) of
-         | SOME (Exception _ _) => T
-         | SOME (Result ret _) => ret <> Loc 1 0
-         | SOME Error => T
-         | NONE => T
-         | _ => F
-  then Fail
-  else
-    case some res.
-      ∃k t r outcome.
-        evaluate (prog, s with clock := k) = (r,t) ∧
-        (case r of
-         | (SOME (FinalFFI e)) => outcome = FFI_outcome e
-         | (SOME (Result _ _)) => outcome = Success
-         | (SOME NotEnoughSpace) => outcome = Resource_limit_hit
-         | _ => F) ∧
-        res = Terminate outcome t.ffi.io_events
-      of
-    | SOME res => res
-    | NONE =>
-      Diverge
-         (build_lprefix_lub
-           (IMAGE (λk. fromList
-              (SND (evaluate (prog,s with clock := k))).ffi.io_events) UNIV))`;
-
-Definition word_lang_safe_for_space_def:
-  word_lang_safe_for_space (s:('a,'c,'ffi) wordSem$state) start =
-    let prog = Call NONE (SOME start) [0] NONE in
-      (!k res t. wordSem$evaluate (prog, s with clock := k) = (res,t) ==>
-        ?max. t.stack_max = SOME max /\ max <= t.stack_limit)
-End
-*)
-
-(* clean up *)
-
-val _ = map delete_binding ["evaluate_AUX_def", "evaluate_primitive_def"];
+Theorem evaluate_ind = REWRITE_RULE [fix_clock_evaluate] evaluate_ind;
+Theorem evaluate_def = REWRITE_RULE [fix_clock_evaluate] evaluate_def;
 
 val _ = export_theory();
