pancake/wheatLangScript.sml
@@ -13,11 +13,8 @@ Datatype:
   exp = Const ('a word)
       | Var num
       | Load exp
-   (* TODISC: crepLang has LoadByte, while wordLand doesn't have, should we have it here?  *)
-   (* | LoadByte exp *)
       | Op binop (exp list)
       | Shift shift exp num
-   (* TODISC: panLang and crepLang has Cmp, wordLang doesnot have it  *)
 End
 
 Datatype:
@@ -26,28 +23,23 @@ Datatype:
        | Store ('a exp) num            (* dest, source *)
        | StoreGlob ('a exp) (5 word)   (* dest, source *)
        | LoadGlob  (5 word) ('a exp)   (* dest, source *)
-    (* TODISC: we should think now whether we need Inst here?
-       also what kind of assembly instructions pancake would support?
-       what is the connection of Inst with Op above? (Arith from Inst uses binop?) *)
-       | Inst ('a inst)
+       | LoadByte num num
        | Seq prog prog
        | If cmp num ('a reg_imm) prog prog
-       | While cmp num ('a reg_imm) prog
+       | Loop num_set prog num_set     (* names in, body, names out *)
        | Break
        | Continue
        | Raise num
        | Return num
        | Tick
+       | Mark prog
        | LocValue num num  (* assign v1 := Loc v2 0 *)
-       | Call (num option) (* return var *)
+       | Call ((num # num_set) option) (* return var *)
               (num option) (* target of call *)
               (num list)   (* arguments *)
               ((num # prog) option)  (* var to store exception, exception-handler code *)
        | FFI string num num num num (* FFI name, conf_ptr, conf_len, array_ptr, array_len, cut-set *)
 End
-
-(* Remove_me_later: word_op and word_sh to be taken from wordLangScript *)
-
 
 Theorem MEM_IMP_exp_size:
    !xs a. MEM a xs ==> (exp_size l a < exp1_size l xs)
@@ -56,7 +48,6 @@ Proof
   \\ REPEAT STRIP_TAC \\ SRW_TAC [] [definition"exp_size_def"]
   \\ RES_TAC \\ DECIDE_TAC
 QED
-
 
 Overload shift = “backend_common$word_shift”
 
